updates

Veritas.Verifier.Merkle.fst
@@ -8,9 +8,9 @@ module BP=Veritas.BinTreePtr
 module E=Veritas.EAC
 
 (* does the log entry update which descendant the value of k points to? *)
-let updates_points_to (e: vlog_entry) (k: merkle_key): bool = 
+let updates_points_to (e: vlog_entry) (k: merkle_key): bool =
   match e with
-  | AddM (k1,_) k2 -> k1 = k || k2 = k  
+  | AddM (k1,_) k2 -> k1 = k || k2 = k
   | _ -> false
 
 let lemma_points_to_unchanged_caseA_root (itsl: TL.eac_log{I.length itsl > 0}) (c:bin_tree_dir):
@@ -19,12 +19,12 @@ let lemma_points_to_unchanged_caseA_root (itsl: TL.eac_log{I.length itsl > 0}) (
                    let ke = V.key_of e in
                    not (updates_points_to e Root) /\ ke <> Root))
         (ensures (let n = I.length itsl in
-                  let itsl' = I.prefix itsl (n - 1) in 
+                  let itsl' = I.prefix itsl (n - 1) in
                   let v = eac_merkle_value itsl Root in
                   let v' = eac_merkle_value itsl' Root in
-                  mv_points_to_none v c && mv_points_to_none v' c || 
-                  mv_points_to_some v c && mv_points_to_some v' c && 
-                  mv_pointed_key v c = mv_pointed_key v' c)) = 
+                  mv_points_to_none v c && mv_points_to_none v' c ||
+                  mv_points_to_some v c && mv_points_to_some v' c &&
+                  mv_pointed_key v c = mv_pointed_key v' c)) =
   let n = I.length itsl in
   let itsl' = I.prefix itsl (n - 1) in
   let e = I.index itsl (n - 1) in
@@ -40,23 +40,23 @@ let lemma_points_to_unchanged_caseA_root (itsl: TL.eac_log{I.length itsl > 0}) (
   (* thread id where element e goes *)
   let tid = thread_id_of itsl (n - 1) in
 
-  if tid = 0 then 
-    lemma_verifier_thread_state_extend itsl (n - 1)  
+  if tid = 0 then
+    lemma_verifier_thread_state_extend itsl (n - 1)
   else
     lemma_verifier_thread_state_extend2 itsl (n - 1) 0
-    
+
 let lemma_points_to_unchanged_caseA (itsl: TL.eac_log{I.length itsl > 0}) (k:merkle_key) (c:bin_tree_dir):
   Lemma (requires (let n = I.length itsl in
                    let e = I.index itsl (n - 1) in
                    let ke = V.key_of e in
                    not (updates_points_to e k) /\ ke <> k ))
         (ensures (let n = I.length itsl in
-                  let itsl' = I.prefix itsl (n - 1) in 
+                  let itsl' = I.prefix itsl (n - 1) in
                   let v = eac_merkle_value itsl k in
                   let v' = eac_merkle_value itsl' k in
-                  mv_points_to_none v c && mv_points_to_none v' c || 
-                  mv_points_to_some v c && mv_points_to_some v' c && 
-                  mv_pointed_key v c = mv_pointed_key v' c)) = 
+                  mv_points_to_none v c && mv_points_to_none v' c ||
+                  mv_points_to_some v c && mv_points_to_some v' c &&
+                  mv_pointed_key v c = mv_pointed_key v' c)) =
    if k = Root then lemma_points_to_unchanged_caseA_root itsl c
    else
 
@@ -67,21 +67,21 @@ let lemma_points_to_unchanged_caseA (itsl: TL.eac_log{I.length itsl > 0}) (k:mer
 
    let es' = TL.eac_state_of_key itsl' k in
    let es = TL.eac_state_of_key itsl k in
-   
+
    lemma_fullprefix_equal itsl;
    lemma_eac_state_of_key_valid itsl k;
    lemma_eac_state_of_key_valid itsl' k;
    lemma_eac_state_same itsl (n - 1) k;
    assert(es <> EACFail);
    assert(es = es');
-   
+
    match es with
-   | EACInit -> 
+   | EACInit ->
      lemma_eac_value_init itsl' k;
      lemma_eac_value_init itsl k
 
-   | EACInStore m v -> 
-   
+   | EACInStore m v ->
+
      (* k is in store of tid after itsl' *)
      let tidk = stored_tid itsl' k in
      assert(store_contains (TL.thread_store itsl' tidk) k);
@@ -104,11 +104,11 @@ let lemma_points_to_unchanged_caseA (itsl: TL.eac_log{I.length itsl > 0}) (k:mer
        //assert(eac_value itsl k = V.stored_value (TL.thread_store itsl tidk) k);
        lemma_eac_value_is_stored_value itsl' k tidk
      )
-       
+
    | EACEvictedMerkle _
-   | EACEvictedBlum _ _ _ ->    
+   | EACEvictedBlum _ _ _ ->
      lemma_eac_value_is_evicted_value itsl k;
-     lemma_eac_value_is_evicted_value itsl' k;     
+     lemma_eac_value_is_evicted_value itsl' k;
      ()
 
 let lemma_points_to_unchanged_evictm (itsl: TL.eac_log {I.length itsl > 0 }) (k: merkle_key) (c: bin_tree_dir):
@@ -116,12 +116,12 @@ let lemma_points_to_unchanged_evictm (itsl: TL.eac_log {I.length itsl > 0 }) (k:
                    let e = I.index itsl (n - 1) in
                    V.key_of e = k /\ EvictM? e))
         (ensures (let n = I.length itsl in
-                  let itsl' = I.prefix itsl (n - 1) in 
+                  let itsl' = I.prefix itsl (n - 1) in
                   let v = eac_merkle_value itsl k in
                   let v' = eac_merkle_value itsl' k in
-                  mv_points_to_none v c && mv_points_to_none v' c || 
-                  mv_points_to_some v c && mv_points_to_some v' c && 
-                  mv_pointed_key v c = mv_pointed_key v' c)) = 
+                  mv_points_to_none v c && mv_points_to_none v' c ||
+                  mv_points_to_some v c && mv_points_to_some v' c &&
+                  mv_pointed_key v c = mv_pointed_key v' c)) =
   let n = I.length itsl in
   let itsl' = I.prefix itsl (n - 1) in
   let e = I.index itsl (n - 1) in
@@ -168,7 +168,7 @@ let lemma_points_to_unchanged_evictm (itsl: TL.eac_log {I.length itsl > 0 }) (k:
 
     lemma_eac_value_is_stored_value itsl' k tid;
     //assert(eac_value itsl' k = V.stored_value st' k);
-    
+
     ()
 
 let lemma_points_to_unchanged_addb (itsl: TL.eac_log {I.length itsl > 0 }) (k: merkle_key) (c: bin_tree_dir):
@@ -176,12 +176,12 @@ let lemma_points_to_unchanged_addb (itsl: TL.eac_log {I.length itsl > 0 }) (k: m
                    let e = I.index itsl (n - 1) in
                    V.key_of e = k /\ AddB? e))
         (ensures (let n = I.length itsl in
-                  let itsl' = I.prefix itsl (n - 1) in 
+                  let itsl' = I.prefix itsl (n - 1) in
                   let v = eac_merkle_value itsl k in
                   let v' = eac_merkle_value itsl' k in
-                  mv_points_to_none v c && mv_points_to_none v' c || 
-                  mv_points_to_some v c && mv_points_to_some v' c && 
-                  mv_pointed_key v c = mv_pointed_key v' c)) = 
+                  mv_points_to_none v c && mv_points_to_none v' c ||
+                  mv_points_to_some v c && mv_points_to_some v' c &&
+                  mv_pointed_key v c = mv_pointed_key v' c)) =
   let n = I.length itsl in
   let itsl' = I.prefix itsl (n - 1) in
   let e = I.index itsl (n - 1) in
@@ -202,14 +202,14 @@ let lemma_points_to_unchanged_addb (itsl: TL.eac_log {I.length itsl > 0 }) (k: m
   (* both es and es' are non-fail states *)
   lemma_eac_state_of_key_valid itsl k;
   lemma_eac_state_of_key_valid itsl' k;
-  // assert(es <> EACFail && es' <> EACFail);  
+  // assert(es <> EACFail && es' <> EACFail);
 
   (* thread store after processing e *)
   let st = TL.thread_store itsl tid in
 
   match e with
   | AddB (_,v) _ _ ->
-    
+
     (* the store contains k after the add *)
     // assert(V.store_contains st k);
 
@@ -222,7 +222,7 @@ let lemma_points_to_unchanged_addb (itsl: TL.eac_log {I.length itsl > 0 }) (k: m
 
     (* eac implies the added value is the value in es' *)
     // assert(v = EACEvictedBlum?.v es');
-    
+
     (* the added value is the value in the store *)
     // assert(V.stored_value st k = v);
 
@@ -233,19 +233,19 @@ let lemma_points_to_unchanged_addb (itsl: TL.eac_log {I.length itsl > 0 }) (k: m
     (* all previous equalities imply eac_value of k is the same before and after e *)
     // assert(eac_value itsl k = eac_value itsl' k);
 
-    ()                  
+    ()
 
 let lemma_points_to_unchanged_evictb (itsl: TL.eac_log {I.length itsl > 0 }) (k: merkle_key) (c: bin_tree_dir):
   Lemma (requires (let n = I.length itsl in
                    let e = I.index itsl (n - 1) in
                    V.key_of e = k /\ EvictB? e))
         (ensures (let n = I.length itsl in
-                  let itsl' = I.prefix itsl (n - 1) in 
+                  let itsl' = I.prefix itsl (n - 1) in
                   let v = eac_merkle_value itsl k in
                   let v' = eac_merkle_value itsl' k in
-                  mv_points_to_none v c && mv_points_to_none v' c || 
-                  mv_points_to_some v c && mv_points_to_some v' c && 
-                  mv_pointed_key v c = mv_pointed_key v' c)) = 
+                  mv_points_to_none v c && mv_points_to_none v' c ||
+                  mv_points_to_some v c && mv_points_to_some v' c &&
+                  mv_pointed_key v c = mv_pointed_key v' c)) =
   let n = I.length itsl in
   let itsl' = I.prefix itsl (n - 1) in
   let e = I.index itsl (n - 1) in
@@ -266,7 +266,7 @@ let lemma_points_to_unchanged_evictb (itsl: TL.eac_log {I.length itsl > 0 }) (k:
   (* both es and es' are non-fail states *)
   lemma_eac_state_of_key_valid itsl k;
   lemma_eac_state_of_key_valid itsl' k;
-  // assert(es <> EACFail && es' <> EACFail);  
+  // assert(es <> EACFail && es' <> EACFail);
 
   (* thread store before processing e *)
   let st' = TL.thread_store itsl' tid in
@@ -300,19 +300,19 @@ let lemma_points_to_unchanged_evictb (itsl: TL.eac_log {I.length itsl > 0 }) (k:
     (* the previous equalities imply, the eac_value of k remains unchanged when processing e *)
     // assert(eac_value itsl k = eac_value itsl' k);
 
-    ()                 
+    ()
 
 let lemma_points_to_unchanged_evictbm (itsl: TL.eac_log {I.length itsl > 0 }) (k: merkle_key) (c: bin_tree_dir):
   Lemma (requires (let n = I.length itsl in
                    let e = I.index itsl (n - 1) in
                    V.key_of e = k /\ EvictBM? e))
         (ensures (let n = I.length itsl in
-                  let itsl' = I.prefix itsl (n - 1) in 
+                  let itsl' = I.prefix itsl (n - 1) in
                   let v = eac_merkle_value itsl k in
                   let v' = eac_merkle_value itsl' k in
-                  mv_points_to_none v c && mv_points_to_none v' c || 
-                  mv_points_to_some v c && mv_points_to_some v' c && 
-                  mv_pointed_key v c = mv_pointed_key v' c)) = 
+                  mv_points_to_none v c && mv_points_to_none v' c ||
+                  mv_points_to_some v c && mv_points_to_some v' c &&
+                  mv_pointed_key v c = mv_pointed_key v' c)) =
   let n = I.length itsl in
   let itsl' = I.prefix itsl (n - 1) in
   let e = I.index itsl (n - 1) in
@@ -333,7 +333,7 @@ let lemma_points_to_unchanged_evictbm (itsl: TL.eac_log {I.length itsl > 0 }) (k
   (* both es and es' are non-fail states *)
   lemma_eac_state_of_key_valid itsl k;
   lemma_eac_state_of_key_valid itsl' k;
-  // assert(es <> EACFail && es' <> EACFail);  
+  // assert(es <> EACFail && es' <> EACFail);
 
   (* thread store before processing e *)
   let st' = TL.thread_store itsl' tid in
@@ -375,12 +375,12 @@ let lemma_points_to_unchanged (itsl: TL.eac_log{I.length itsl > 0}) (k:merkle_ke
                    let e = I.index itsl (n - 1) in
                    not (updates_points_to e k)))
         (ensures (let n = I.length itsl in
-                  let itsl' = I.prefix itsl (n - 1) in 
+                  let itsl' = I.prefix itsl (n - 1) in
                   let v = eac_merkle_value itsl k in
                   let v' = eac_merkle_value itsl' k in
-                  mv_points_to_none v c && mv_points_to_none v' c || 
-                  mv_points_to_some v c && mv_points_to_some v' c && 
-                  mv_pointed_key v c = mv_pointed_key v' c)) = 
+                  mv_points_to_none v c && mv_points_to_none v' c ||
+                  mv_points_to_some v c && mv_points_to_some v' c &&
+                  mv_pointed_key v c = mv_pointed_key v' c)) =
   let n = I.length itsl in
   let itsl' = I.prefix itsl (n - 1) in
   let e = I.index itsl (n - 1) in
@@ -388,14 +388,14 @@ let lemma_points_to_unchanged (itsl: TL.eac_log{I.length itsl > 0}) (k:merkle_ke
 
   if ke <> k then
     lemma_points_to_unchanged_caseA itsl k c
-  else ( 
+  else (
     match e with
     | Get _ _ -> ()                 (* k is a merkle key *)
     | Put _ _ -> ()                 (* k is a merkle key *)
     | AddM _ _ -> ()                 (* update_points_to ... => contradiction *)
     | EvictM _ _ -> lemma_points_to_unchanged_evictm itsl k c
     | AddB _ _ _ -> lemma_points_to_unchanged_addb itsl k c
-    | EvictB _ _ -> lemma_points_to_unchanged_evictb itsl k c    
+    | EvictB _ _ -> lemma_points_to_unchanged_evictb itsl k c
     | EvictBM _ _ _ -> lemma_points_to_unchanged_evictbm itsl k c
   )
 
@@ -405,14 +405,14 @@ let lemma_eac_value_empty_or_points_to_desc_addmA
   (c:bin_tree_dir):
   Lemma (requires (let n = I.length itsl in
                    let itsl' = I.prefix itsl (n - 1) in
-                   let e = I.index itsl (n - 1) in                   
+                   let e = I.index itsl (n - 1) in
                    let v' = eac_merkle_value itsl' k in
                    V.key_of e = k /\ AddM? e /\
                    (mv_points_to_none v' c \/
                     mv_points_to_some v' c /\ is_desc (mv_pointed_key v' c) (child c k))))
          (ensures (let v = eac_merkle_value itsl k in
                    mv_points_to_none v c \/
-                   mv_points_to_some v c /\ is_desc (mv_pointed_key v c) (child c k))) = 
+                   mv_points_to_some v c /\ is_desc (mv_pointed_key v c) (child c k))) =
   let n = I.length itsl in
   let itsl' = I.prefix itsl (n - 1) in
   let e = I.index itsl (n - 1) in
@@ -433,7 +433,7 @@ let lemma_eac_value_empty_or_points_to_desc_addmA
   (* both es and es' are non-fail states *)
   lemma_eac_state_of_key_valid itsl k;
   lemma_eac_state_of_key_valid itsl' k;
-  // assert(es <> EACFail && es' <> EACFail);  
+  // assert(es <> EACFail && es' <> EACFail);
 
   (* thread store before processing e *)
   let st' = TL.thread_store itsl' tid in
@@ -450,15 +450,15 @@ let lemma_eac_value_empty_or_points_to_desc_addmA
     let c' = desc_dir k k' in
     let dh' = desc_hash_dir v' c' in
     match dh' with
-    | Empty -> 
+    | Empty ->
       // assert(v = init_value k);
-      // assert(V.store_contains st k);      
+      // assert(V.store_contains st k);
       // assert(V.stored_value st k = v);
       lemma_eac_value_is_stored_value itsl k tid
-      
+
     | Desc k2 _ _ ->
       if k2 = k then (
-        // assert(V.stored_value st k = v);        
+        // assert(V.stored_value st k = v);
         lemma_eac_value_is_stored_value itsl k tid;
         // assert(eac_value itsl k = v);
 
@@ -473,25 +473,25 @@ let lemma_eac_value_empty_or_points_to_desc_addmA
           ()
         )
       )
-      else 
+      else
         //assert(v = init_value k);
         //assert(is_proper_desc k2 k);
         lemma_eac_value_is_stored_value itsl k tid
-      
+
 let lemma_eac_value_empty_or_points_to_desc_addmB
   (itsl: TL.eac_log {I.length itsl > 0})
   (k:merkle_key)
   (c:bin_tree_dir):
   Lemma (requires (let n = I.length itsl in
                    let itsl' = I.prefix itsl (n - 1) in
-                   let e = I.index itsl (n - 1) in                   
+                   let e = I.index itsl (n - 1) in
                    let v' = eac_merkle_value itsl' k in
                    AddM? e /\ AddM?.k' e  = k /\
                    (mv_points_to_none v' c \/
                     mv_points_to_some v' c /\ is_desc (mv_pointed_key v' c) (child c k))))
          (ensures (let v = eac_merkle_value itsl k in
                    mv_points_to_none v c \/
-                   mv_points_to_some v c /\ is_desc (mv_pointed_key v c) (child c k))) = 
+                   mv_points_to_some v c /\ is_desc (mv_pointed_key v c) (child c k))) =
   let n = I.length itsl in
   let itsl' = I.prefix itsl (n - 1) in
   let e = I.index itsl (n - 1) in
@@ -512,14 +512,14 @@ let lemma_eac_value_empty_or_points_to_desc_addmB
   (* both es and es' are non-fail states *)
   lemma_eac_state_of_key_valid itsl k;
   lemma_eac_state_of_key_valid itsl' k;
-  // assert(es <> EACFail && es' <> EACFail);  
+  // assert(es <> EACFail && es' <> EACFail);
 
   (* thread store before processing e *)
   // let st' = TL.thread_store itsl' tid in
   (* thread store after processing e *)
   // let st = TL.thread_store itsl tid in
   match e with
-  | AddM (k1,v1) _ ->                     
+  | AddM (k1,v1) _ ->
     (* verifier checks *)
     // assert(is_proper_desc k1 k);
     // assert(V.store_contains st' k);
@@ -527,7 +527,7 @@ let lemma_eac_value_empty_or_points_to_desc_addmB
     // let c' = desc_dir k1 k in
     // let dh' = desc_hash_dir v' c' in
     // let h1 = hashfn v1 in
-  
+
     (* store contains k after processing e *)
     // assert(V.store_contains st k);
     lemma_eac_value_is_stored_value itsl k tid;
@@ -542,7 +542,7 @@ let rec lemma_eac_value_empty_or_points_to_desc
         (ensures (let v = eac_merkle_value itsl k in
                   mv_points_to_none v c \/
                   mv_points_to_some v c /\ is_desc (mv_pointed_key v c) (child c k)))
-        (decreases (I.length itsl)) = 
+        (decreases (I.length itsl)) =
   let n = I.length itsl in
 
   if n = 0 then (
@@ -553,7 +553,7 @@ let rec lemma_eac_value_empty_or_points_to_desc
     else
       lemma_eac_value_init itsl k
   )
-  else 
+  else
     let itsl' = I.prefix itsl (n - 1) in
     let e = I.index itsl (n - 1) in
 
@@ -566,16 +566,16 @@ let rec lemma_eac_value_empty_or_points_to_desc
         assert(k1 = k || k2 = k);
 
 
-        if k1 = k then           
-          lemma_eac_value_empty_or_points_to_desc_addmA itsl k c        
+        if k1 = k then
+          lemma_eac_value_empty_or_points_to_desc_addmA itsl k c
         else
           lemma_eac_value_empty_or_points_to_desc_addmB itsl k c
     )
-    else 
+    else
       lemma_points_to_unchanged itsl k c
-      
+
 let eac_ptrfn_aux (itsl: TL.eac_log) (n:bin_tree_node) (c:bin_tree_dir):
-  option (d:bin_tree_node{is_desc d (child c n)}) = 
+  option (d:bin_tree_node{is_desc d (child c n)}) =
   if depth n >= key_size then None
   else (
     let ev = to_merkle_value (eac_value itsl n) in
@@ -595,10 +595,10 @@ let lemma_eac_ptrfn (itsl: TL.eac_log) (k: merkle_key) (c:bin_tree_dir) :
   Lemma (requires True)
         (ensures (let pf = eac_ptrfn itsl in
                   let mv = eac_merkle_value itsl k in
-                  mv_points_to_none mv c /\ pf k c = None \/                   
+                  mv_points_to_none mv c /\ pf k c = None \/
                   mv_points_to_some mv c /\ is_desc (mv_pointed_key mv c) (child c k) /\
                   pf k c = Some (mv_pointed_key mv c)))
-        [SMTPat (eac_ptrfn itsl k c)] = 
+        [SMTPat (eac_ptrfn itsl k c)] =
   let pf = eac_ptrfn itsl in
   let mv = eac_merkle_value itsl k in
   if mv_points_to_none mv c then ()
@@ -608,12 +608,12 @@ let lemma_eac_ptrfn (itsl: TL.eac_log) (k: merkle_key) (c:bin_tree_dir) :
     ()
   )
 
-let root_reachable (itsl: TL.eac_log) (k:key): bool = 
+let root_reachable (itsl: TL.eac_log) (k:key): bool =
   let pf = eac_ptrfn itsl in
   BP.root_reachable pf k
 
 (* only merkle adds may change the pointer function *)
-let may_change_ptrfn (e: vlog_entry): bool = 
+let may_change_ptrfn (e: vlog_entry): bool =
   match e with
   | AddM _ _ -> true
   | _ -> false
@@ -623,9 +623,9 @@ let lemma_ptrfn_unchanged_aux (itsl: TL.eac_log {I.length itsl > 0}) (k:merkle_k
                    let e = I.index itsl (n - 1) in
                    not (may_change_ptrfn e)))
         (ensures (let n = I.length itsl in
-                  let itsl' = I.prefix itsl (n - 1) in        
-                  eac_ptrfn itsl k c = eac_ptrfn itsl' k c)) 
-        [SMTPat (eac_ptrfn itsl k c)] =                  
+                  let itsl' = I.prefix itsl (n - 1) in
+                  eac_ptrfn itsl k c = eac_ptrfn itsl' k c))
+        [SMTPat (eac_ptrfn itsl k c)] =
   lemma_points_to_unchanged itsl k c;
   lemma_eac_ptrfn itsl k c
 
@@ -635,7 +635,7 @@ let lemma_ptrfn_unchanged (itsl: TL.eac_log {I.length itsl > 0}):
                    not (may_change_ptrfn e)))
         (ensures (let n = I.length itsl in
                   let itsl' = I.prefix itsl (n - 1) in
-                  feq_ptrfn (eac_ptrfn itsl) (eac_ptrfn itsl'))) =                     
+                  feq_ptrfn (eac_ptrfn itsl) (eac_ptrfn itsl'))) =
   ()
 
 let lemma_ptrfn_unchanged_implies_initness_unchanged (itsl: TL.eac_log {I.length itsl > 0}) (k:key {k <> Root}):
@@ -645,19 +645,19 @@ let lemma_ptrfn_unchanged_implies_initness_unchanged (itsl: TL.eac_log {I.length
                    not (may_change_ptrfn e)))
          (ensures (let n = I.length itsl in
                    let itsl' = I.prefix itsl (n - 1) in
-                   is_eac_state_init itsl' k = is_eac_state_init itsl k)) = 
+                   is_eac_state_init itsl' k = is_eac_state_init itsl k)) =
   let n = I.length itsl in
-  let itsl' = I.prefix itsl (n - 1) in                   
+  let itsl' = I.prefix itsl (n - 1) in
   let es' = TL.eac_state_of_key itsl' k in
   let es = TL.eac_state_of_key itsl k in
-  
+
   lemma_eac_state_of_key_valid itsl k;
   lemma_eac_state_of_key_valid itsl' k;
-  // assert(es <> EACFail && es' <> EACFail);  
+  // assert(es <> EACFail && es' <> EACFail);
 
   (* nothing to prove if es and es' are equal *)
   if es = es' then ()
-  
+
   (* also nothing to prove if neither es es' are EACInit *)
   else if es <> EACInit && es' <> EACInit then ()
 
@@ -676,17 +676,17 @@ let lemma_ptrfn_unchanged_implies_initness_unchanged (itsl: TL.eac_log {I.length
   )
   else (
     assert(es' = EACInit && es <> EACInit);
-    let e = I.index itsl (n - 1) in       
+    let e = I.index itsl (n - 1) in
     let ee = TL.vlog_entry_ext_at itsl (n - 1) in
-    
+
     lemma_fullprefix_equal itsl;
 
     (* if the key of the last entry is k, then we know tha es is obtained from es' by eac_add *)
     (* this would imply that e is an AddM providing a contradiction (not (may_change_ptrfn)) *)
-    if V.key_of e = k then 
-      
+    if V.key_of e = k then
+
       lemma_eac_state_transition itsl (n - 1)
-      // assert(es = eac_add ee es');      
+      // assert(es = eac_add ee es');
       // assert(AddM? e);
 
     (* if the key of e is not k, the es = es', which provides a contradiction *)
@@ -699,14 +699,14 @@ let lemma_not_init_equiv_root_reachable_extend_ptrfn_unchanged (itsl: TL.eac_log
                    let e = I.index itsl (n - 1) in
                    let itsl' = I.prefix itsl (n - 1) in
                    not (may_change_ptrfn e) /\
-                   (not (is_eac_state_init itsl' k) <==> root_reachable itsl' k)))                   
-        (ensures (not (is_eac_state_init itsl k) <==> root_reachable itsl k)) =  
+                   (not (is_eac_state_init itsl' k) <==> root_reachable itsl' k)))
+        (ensures (not (is_eac_state_init itsl k) <==> root_reachable itsl k)) =
  let n = I.length itsl in
  let pf = eac_ptrfn itsl in
- let itsl' = I.prefix itsl (n - 1) in 
+ let itsl' = I.prefix itsl (n - 1) in
  let pf' = eac_ptrfn itsl' in
-  
- (* the pointer functions of itsl and itsl' are the same, so root_reachability is unaffected *)        
+
+ (* the pointer functions of itsl and itsl' are the same, so root_reachability is unaffected *)
  lemma_ptrfn_unchanged itsl;
  lemma_reachable_feq pf pf' k Root;
  assert(root_reachable itsl k = root_reachable itsl' k);
@@ -715,21 +715,21 @@ let lemma_not_init_equiv_root_reachable_extend_ptrfn_unchanged (itsl: TL.eac_log
  lemma_ptrfn_unchanged_implies_initness_unchanged itsl k
 
 (* three type of edge additions due to AddM (k,_) k' *)
-type addm_type = 
+type addm_type =
   | NoNewEdge         (* common case: no new added; k' points k *)
   | NewEdge           (* new edge added: k' points to none along k direction *)
   | CutEdge           (* cut an existing edge: k' points to k2, is_proper_desc k2 k *)
 
 (* type of an addm based on the edge additions it induces *)
-let type_of_addm (itsl: TL.eac_log) 
-                 (i: I.seq_index itsl { AddM? (I.index itsl i)}): addm_type = 
-  let tid = TL.thread_id_of itsl i in                 
-  let e = I.index itsl i in           
-  
+let type_of_addm (itsl: TL.eac_log)
+                 (i: I.seq_index itsl { AddM? (I.index itsl i)}): addm_type =
+  let tid = TL.thread_id_of itsl i in
+  let e = I.index itsl i in
+
   let lpre = I.prefix itsl i in
   let vspre = TL.thread_state lpre tid in
   let stpre = TL.thread_store lpre tid in
-  
+
   let lpost = I.prefix itsl (i + 1) in
   let vspost = TL.thread_state lpost tid in
   let stpost = TL.thread_store lpost tid in
@@ -738,7 +738,7 @@ let type_of_addm (itsl: TL.eac_log)
   assert(vspost == t_verify_step vspre e);
 
   match e with
-  | AddM (k,_) k' ->    
+  | AddM (k,_) k' ->
     let v' = to_merkle_value (V.stored_value stpre k') in
     let d = desc_dir k k' in
     let dh' = desc_hash_dir v' d in
@@ -748,30 +748,30 @@ let type_of_addm (itsl: TL.eac_log)
                      else CutEdge
 
 (* direction of the cut_edge from the added key *)
-let cut_edge_dir 
-  (itsl: TL.eac_log) 
-  (i: I.seq_index itsl {AddM? (I.index itsl i) /\ type_of_addm itsl i = CutEdge}): bin_tree_dir = 
-  let tid = TL.thread_id_of itsl i in                 
-  let e = I.index itsl i in             
+let cut_edge_dir
+  (itsl: TL.eac_log)
+  (i: I.seq_index itsl {AddM? (I.index itsl i) /\ type_of_addm itsl i = CutEdge}): bin_tree_dir =
+  let tid = TL.thread_id_of itsl i in
+  let e = I.index itsl i in
   let lpre = I.prefix itsl i in
 
-  let stpre = TL.thread_store lpre tid in  
+  let stpre = TL.thread_store lpre tid in
   lemma_verifier_thread_state_extend itsl i;
 
   match e with
-  | AddM (k,_) k' ->    
+  | AddM (k,_) k' ->
     let v' = to_merkle_value (V.stored_value stpre k') in
     let d = desc_dir k k' in
     let dh' = desc_hash_dir v' d in
     match dh' with
-    | Desc k2 _ _ -> 
+    | Desc k2 _ _ ->
       desc_dir k2 k
 
 (* direction of k' -> k in an AddM (k,_) k' *)
 let add_dir
   (itsl: TL.eac_log)
-  (i: I.seq_index itsl {AddM? (I.index itsl i)}): 
-    (c:bin_tree_dir{ 
+  (i: I.seq_index itsl {AddM? (I.index itsl i)}):
+    (c:bin_tree_dir{
       let e = I.index itsl i in
       let k = V.key_of e in
       let k' = AddM?.k' e in
@@ -809,7 +809,7 @@ let lemma_addm_anc_points_to (itsl: TL.eac_log {I.length itsl > 0}):
   let pf' = eac_ptrfn itsl' in
   let c = add_dir itsl (n - 1) in
   let k = V.key_of e in
-  let oc = other_dir c in  
+  let oc = other_dir c in
   lemma_fullprefix_equal itsl;
   lemma_verifier_thread_state_extend itsl (n-1);
 
@@ -830,13 +830,13 @@ let lemma_addm_desc_points_to (itsl: TL.eac_log {I.length itsl > 0}):
                   let k' = AddM?.k' e in
                   let pf = eac_ptrfn itsl in
                   let pf' = eac_ptrfn itsl' in
-                  is_proper_desc k k' /\ 
+                  is_proper_desc k k' /\
                   (type_of_addm itsl (n - 1) = NewEdge /\ BP.points_to_none pf k) \/
                   (type_of_addm itsl (n - 1) = NoNewEdge /\ pf k Left = pf' k Left /\ pf k Right = pf' k Right) \/
-                  (type_of_addm itsl (n - 1) = CutEdge /\ 
+                  (type_of_addm itsl (n - 1) = CutEdge /\
                    points_to_some pf' k' (add_dir itsl (n - 1)) /\
                    points_to_some pf k (cut_edge_dir itsl (n - 1)) /\
-                   pointed_node pf' k' (add_dir itsl (n - 1)) = 
+                   pointed_node pf' k' (add_dir itsl (n - 1)) =
                    pointed_node pf k (cut_edge_dir itsl (n - 1))))) =
   let n = I.length itsl in
   let tid = TL.thread_id_of itsl (n-1) in
@@ -870,30 +870,30 @@ let lemma_addm_desc_points_to (itsl: TL.eac_log {I.length itsl > 0}):
     match dh' with
     | Empty -> ()
     | Desc k2 _ _ ->
-      if k2 = k then 
-        if es' = EACInit then 
-          lemma_eac_value_init itsl' k          
-        else     
-          lemma_eac_value_is_evicted_value itsl' k              
+      if k2 = k then
+        if es' = EACInit then
+          lemma_eac_value_init itsl' k
+        else
+          lemma_eac_value_is_evicted_value itsl' k
       else ()
-  
-let not_init_equiv_root_reachable (itsl: TL.eac_log) (k:key): bool = 
+
+let not_init_equiv_root_reachable (itsl: TL.eac_log) (k:key): bool =
   k = Root ||
   is_eac_state_init itsl k && not (root_reachable itsl k) ||
   not (is_eac_state_init itsl k) && root_reachable itsl k
 
+(* if the AddM type is NoNewEdge, then the ptr function remains unchanged after processing this entry *)
 let lemma_ptrfn_unchanged_addm_nonewedge (itsl: TL.eac_log {I.length itsl > 0}):
   Lemma (requires (let n = I.length itsl in
-                   let itsl' = I.prefix itsl (n - 1) in
                    let e = I.index itsl (n - 1) in
-                   AddM? e /\ 
+                   AddM? e /\
                    type_of_addm itsl (n - 1) = NoNewEdge))
-         (ensures (let n = I.length itsl in                   
-                   let itsl' = I.prefix itsl (n - 1) in                   
-                   feq_ptrfn (eac_ptrfn itsl) (eac_ptrfn itsl'))) = 
+         (ensures (let n = I.length itsl in
+                   let itsl' = I.prefix itsl (n - 1) in
+                   feq_ptrfn (eac_ptrfn itsl) (eac_ptrfn itsl'))) =
   let n = I.length itsl in
   let pf = eac_ptrfn itsl in
-  let tid = TL.thread_id_of itsl (n-1) in  
+  let tid = TL.thread_id_of itsl (n-1) in
   let itsl' = I.prefix itsl (n - 1) in
   let pf' = eac_ptrfn itsl' in
   let e = I.index itsl (n - 1) in
@@ -913,22 +913,104 @@ let lemma_ptrfn_unchanged_addm_nonewedge (itsl: TL.eac_log {I.length itsl > 0}):
   let aux (k1:merkle_key) (c1:bin_tree_dir):
     Lemma (requires True)
           (ensures (pf k1 c1 = pf' k1 c1))
-          [SMTPat (pf k1 c1)] = 
+          [SMTPat (pf k1 c1)] =
     if depth k1 >= key_size then ()
-    else if k1 = k then lemma_addm_desc_points_to itsl      
-    else if k1 = k' then ()        
-    else lemma_points_to_unchanged itsl k1 c1         
-  in      
+    else if k1 = k then lemma_addm_desc_points_to itsl
+    else if k1 = k' then ()
+    else lemma_points_to_unchanged itsl k1 c1
+  in
     ()
 
-let lemma_not_init_equiv_root_reachable_extend_addm_key 
+let lemma_ptrfn_extend_addm_newedge (itsl: TL.eac_log {I.length itsl > 0}):
+  Lemma (requires (let n = I.length itsl in
+                   let e = I.index itsl (n - 1) in
+                   let itsl' = I.prefix itsl (n - 1) in
+                   let pf' = eac_ptrfn itsl' in                   
+                   AddM? e /\
+                   type_of_addm itsl (n - 1) = NewEdge /\
+                   BP.root_reachable pf' (AddM?.k' e)))
+        (ensures (let n = I.length itsl in
+                  let e = I.index itsl (n - 1) in
+                  let itsl' = I.prefix itsl (n - 1) in
+                  let k = V.key_of e in
+                  let k' = AddM?.k' e in
+                  let c = add_dir itsl (n - 1) in
+                  let pf = eac_ptrfn itsl in
+                  let pf' = eac_ptrfn itsl' in
+                  points_to_none pf' k /\
+                  not (points_to_some pf' k' c) /\                  
+                  feq_ptrfn pf (extend_ptrfn pf' k k'))) =
+  let n = I.length itsl in
+  let e = I.index itsl (n - 1) in
+  let tid = TL.thread_id_of itsl (n-1) in  
+  let k = V.key_of e in
+  let k' = AddM?.k' e in
+  let c = add_dir itsl (n - 1) in
+  let pf = eac_ptrfn itsl in
+  let es = TL.eac_state_of_key itsl k in
+  
+  let itsl' = I.prefix itsl (n - 1) in
+  let pf' = eac_ptrfn itsl' in
+  let es' = TL.eac_state_of_key itsl' k in
+
+  lemma_fullprefix_equal itsl;
+  lemma_verifier_thread_state_extend itsl (n-1);
+  lemma_eac_state_of_key_valid itsl k;
+  lemma_eac_state_of_key_valid itsl' k;
+  lemma_eac_state_transition itsl (n - 1);
+  assert(es <> EACFail && es' <> EACFail);
+
+  lemma_addm_anc_points_to itsl;
+
+  match e with
+  | AddM (_,v) _ ->
+    assert(v = init_value k);
+
+    lemma_eac_value_is_stored_value itsl' k' tid;
+    lemma_eac_ptrfn itsl' k' c;
+    assert(not (points_to_some pf' k' c));
+
+    lemma_instore_implies_eac_state_instore itsl k tid;
+    assert(EACInStore? es);
+    assert(es' = EACInit || EACEvictedMerkle? es');
+
+    (* in pf', k points to none *)
+    let lemma_k_points_to_none():
+      Lemma (points_to_none pf' k) = 
+      if es' = EACInit then
+        lemma_eac_value_init itsl' k
+      else
+        lemma_eac_value_is_evicted_value itsl' k
+    in 
+    lemma_k_points_to_none();
+    lemma_eac_value_is_stored_value itsl k tid;
+
+    let pf'e = extend_ptrfn pf' k k' in
+    let aux (k1:bin_tree_node) (c1:bin_tree_dir):
+      Lemma (requires True)
+            (ensures (pf k1 c1 = pf'e k1 c1))
+            [SMTPat (pf k1 c1)] =  
+      if depth k1 >= key_size then ()            
+      else if k1 = k then ()
+      else if k1 = k' then
+        ()
+      else
+        lemma_points_to_unchanged itsl k1 c1
+    in
+
+    ()
+
+
+
+
+let lemma_not_init_equiv_root_reachable_extend_addm_key
   (itsl: TL.eac_log {I.length itsl > 0}) (k: key {k <> Root}):
   Lemma (requires (let n = I.length itsl in
                    let itsl' = I.prefix itsl (n - 1) in
                    let e = I.index itsl (n - 1) in
                    AddM? e /\ V.key_of e = k /\
                    not_init_equiv_root_reachable itsl' (AddM?.k' e)))
-        (ensures (not_init_equiv_root_reachable itsl k)) = 
+        (ensures (not_init_equiv_root_reachable itsl k)) =
   let n = I.length itsl in
   let itsl' = I.prefix itsl (n - 1) in
   let e = I.index itsl (n - 1) in
@@ -938,15 +1020,15 @@ let lemma_not_init_equiv_root_reachable_extend_addm_key
   match e with
   | AddM (k,_) k' ->
 
-         
+
 
     admit()
-                                     
+
 (* a key is root reachable iff its eac_state is not EACInit *)
 let rec lemma_not_init_equiv_root_reachable (itsl: TL.eac_log) (k:key):
-  Lemma (requires True) 
+  Lemma (requires True)
         (ensures (not_init_equiv_root_reachable itsl k))
-        (decreases (I.length itsl)) = 
+        (decreases (I.length itsl)) =
   let n = I.length itsl in
   let es = TL.eac_state_of_key itsl k in
   let pf = eac_ptrfn itsl in
@@ -957,10 +1039,10 @@ let rec lemma_not_init_equiv_root_reachable (itsl: TL.eac_log) (k:key):
     lemma_init_state_empty itsl k;
     assert(es = EACInit);
 
-    (* we need to prove not (root_reachable ...) *)    
+    (* we need to prove not (root_reachable ...) *)
     lemma_eac_value_root_init itsl Root;
     assert(eac_value itsl Root = init_value Root);
-    
+
     (* root is a proper ancestor of k *)
     lemma_root_is_univ_ancestor k;
     assert(is_proper_desc k Root);
@@ -976,10 +1058,10 @@ let rec lemma_not_init_equiv_root_reachable (itsl: TL.eac_log) (k:key):
     lemma_non_reachable_desc_of_none pf k Root
   )
   else (
-    let tid = TL.thread_id_of itsl (n - 1) in  
+    let tid = TL.thread_id_of itsl (n - 1) in
     let e = I.index itsl (n - 1) in
-    let vs = TL.thread_state itsl tid in    
-    
+    let vs = TL.thread_state itsl tid in
+
     let itsl' = I.prefix itsl (n - 1) in
     let es' = TL.eac_state_of_key itsl' k in
     let vs' = TL.thread_state itsl' tid in
@@ -988,11 +1070,11 @@ let rec lemma_not_init_equiv_root_reachable (itsl: TL.eac_log) (k:key):
     lemma_not_init_equiv_root_reachable itsl' k;
 
     match e with
-    | AddM (k1,v1) k2 -> 
+    | AddM (k1,v1) k2 ->
       lemma_not_init_equiv_root_reachable itsl' k2;
-      if k1 = k then 
-        lemma_not_init_equiv_root_reachable_extend_addm_key itsl k      
-      else           
+      if k1 = k then
+        lemma_not_init_equiv_root_reachable_extend_addm_key itsl k
+      else
         admit()
     | _ ->
       assert(not (may_change_ptrfn e));
@@ -1001,17 +1083,17 @@ let rec lemma_not_init_equiv_root_reachable (itsl: TL.eac_log) (k:key):
 
 let rec first_root_reachable_ancestor (itsl: TL.eac_log) (k:key):
   Tot (k':key{root_reachable itsl k' /\
-              is_desc k k'}) 
-  (decreases (depth k)) = 
+              is_desc k k'})
+  (decreases (depth k)) =
   let pf = eac_ptrfn itsl in
-  
+
   if root_reachable itsl k then (
     lemma_desc_reflexive k;
     k
   )
   else (
     (* root is reachable from itself *)
-    lemma_reachable_reflexive pf Root; 
+    lemma_reachable_reflexive pf Root;
 
     (* since k is not root_reachable, k cannot be Root *)
     assert(k <> Root);
@@ -1021,7 +1103,7 @@ let rec first_root_reachable_ancestor (itsl: TL.eac_log) (k:key):
 
     (* recurse ... *)
     let k' = first_root_reachable_ancestor itsl kp in
-    
+
     lemma_parent_ancestor k;
     lemma_desc_transitive k kp k';
     k'
@@ -1029,20 +1111,20 @@ let rec first_root_reachable_ancestor (itsl: TL.eac_log) (k:key):
 
 (* the ancestor who holds the proof of the value of key k *)
 let proving_ancestor (itsl: TL.eac_log) (k:key{k <> Root}):
-  k':key{is_proper_desc k k'} = 
+  k':key{is_proper_desc k k'} =
   let pf = eac_ptrfn itsl in
   lemma_not_init_equiv_root_reachable itsl k;
-  
-  if root_reachable itsl k then 
+
+  if root_reachable itsl k then
     //assert(not (is_eac_state_init itsl k));
-    prev_in_path pf k Root  
+    prev_in_path pf k Root
   else first_root_reachable_ancestor itsl k
 
 let lemma_proving_ancestor_root_reachable (itsl: TL.eac_log) (k:key{k <> Root}):
   Lemma (let k' = proving_ancestor itsl k in
          root_reachable itsl k') = admit()
 
-let lemma_proving_ancestor_greatest_depth (itsl: TL.eac_log) (k:key{k <> Root}) (k2: key{is_proper_desc k k2}):  
+let lemma_proving_ancestor_greatest_depth (itsl: TL.eac_log) (k:key{k <> Root}) (k2: key{is_proper_desc k k2}):
   Lemma (requires (root_reachable itsl k2))
         (ensures  (let k' = proving_ancestor itsl k in
                    depth k2 <= depth k')) = admit()
@@ -1053,8 +1135,8 @@ let lemma_proving_ancestor_points_to_self (itsl: TL.eac_log) (k:key{k <> Root}):
         (ensures (mv_points_to (eac_merkle_value itsl (proving_ancestor itsl k))
                                (desc_dir k (proving_ancestor itsl k))
                                k)) =
-  admit()                               
-   
+  admit()
+
 (* before the first add the proving ancestor points to none or to a key that is not an ancestor *)
 let lemma_proving_ancestor_initial (itsl: TL.eac_log) (k:key{k <> Root}):
   Lemma (requires (is_eac_state_init itsl k))
@@ -1063,14 +1145,14 @@ let lemma_proving_ancestor_initial (itsl: TL.eac_log) (k:key{k <> Root}):
                   let c = desc_dir k k' in
                   mv_points_to_none v' c \/
                   not (is_desc k (mv_pointed_key v' c)))) =
-  let pf = eac_ptrfn itsl in                  
-  let k' = proving_ancestor itsl k in                  
+  let pf = eac_ptrfn itsl in
+  let k' = proving_ancestor itsl k in
   let v' = eac_merkle_value itsl k' in
   let c = desc_dir k k' in
 
   (* k' is root reachable *)
   lemma_proving_ancestor_root_reachable itsl k;
-  assert(root_reachable itsl k');  
+  assert(root_reachable itsl k');
 
   (* k is not root reachable since it is in initial state *)
   lemma_not_init_equiv_root_reachable itsl k;
@@ -1088,7 +1170,7 @@ let lemma_proving_ancestor_initial (itsl: TL.eac_log) (k:key{k <> Root}):
     //assert(is_desc k2 (child c k'));
     lemma_proper_desc_transitive1 k2 (child c k') k';
     //assert(is_proper_desc k2 k');
-    
+
     (* since Root -> k' path exists, k' -> k2 edge exists, Root -> k2 path exists *)
     //assert(points_to pf k2 k');
     lemma_points_to_reachable pf k2 k';
@@ -1101,13 +1183,13 @@ let lemma_proving_ancestor_initial (itsl: TL.eac_log) (k:key{k <> Root}):
       (* if k = k2, we have a contradiction since k is root_reachable *)
       if k = k2 then ()
 
-      (* if k2 <> k, then k2 is a proper ancestor of k, which is a contradiction since k' is the 
+      (* if k2 <> k, then k2 is a proper ancestor of k, which is a contradiction since k' is the
        * first such ancestor going up from k *)
-      else 
-        //assert(is_proper_desc k k2);        
+      else
+        //assert(is_proper_desc k k2);
         lemma_proving_ancestor_greatest_depth itsl k k2
         //assert(depth k2 <= depth k');
-      
+
     (* nothing to prove if k is not a descendant of k2 *)
     else ()
 
@@ -1115,15 +1197,15 @@ let lemma_proving_ancestor_initial (itsl: TL.eac_log) (k:key{k <> Root}):
 let lemma_proving_ancestor_has_hash (itsl: TL.eac_log) (k:key{k<> Root}):
   Lemma (requires (is_eac_state_evicted_merkle itsl k))
         (ensures (mv_pointed_hash (eac_merkle_value itsl (proving_ancestor itsl k))
-                                  (desc_dir k (proving_ancestor itsl k)) = 
-                  hashfn (eac_value itsl k))) = 
-  admit()                  
+                                  (desc_dir k (proving_ancestor itsl k)) =
+                  hashfn (eac_value itsl k))) =
+  admit()
 
 (* when evicted as blum the proving ancestor contains a bit indicating the eviction *)
 let lemma_proving_ancestor_blum_bit (itsl: TL.eac_log) (k:key{k <> Root}):
   Lemma (requires (TL.is_eac_state_evicted itsl k))
         (ensures (mv_evicted_to_blum (eac_merkle_value itsl (proving_ancestor itsl k))
-                                     (desc_dir k (proving_ancestor itsl k)) = 
+                                     (desc_dir k (proving_ancestor itsl k)) =
                   is_eac_state_evicted_blum itsl k)) = admit()
 
 (* if a key is the store of any verifier, then it is root reachable *)
@@ -1131,11 +1213,11 @@ let lemma_instore_implies_root_reachable (itsl: TL.eac_log) (k:key) (tid:valid_t
   Lemma (requires (store_contains (TL.thread_store itsl tid) k))
         (ensures (root_reachable itsl k)) = admit()
 
-(* 
- * Helper lemma for lemma_addm_ancestor_is_proving 
+(*
+ * Helper lemma for lemma_addm_ancestor_is_proving
  *
- * the last log entry is AddM (k,_) k' such that k is root_reachable and 
- * eac_value of k' along the direction of k is emtpy. 
+ * the last log entry is AddM (k,_) k' such that k is root_reachable and
+ * eac_value of k' along the direction of k is emtpy.
  * We prove that this produces a contradiction.
  *)
 let lemma_addm_ancestor_is_proving_caseA (itsl: its_log {I.length itsl > 0}):
@@ -1209,7 +1291,7 @@ let lemma_addm_ancestor_is_proving_caseB (itsl: its_log {I.length itsl > 0}):
                   let e = I.index itsl (n - 1) in
                   let itsl' = I.prefix itsl (n - 1) in
                   let k = V.key_of e in
-                  AddM?.k' e = proving_ancestor itsl' k)) = 
+                  AddM?.k' e = proving_ancestor itsl' k)) =
   let n = I.length itsl in
   let e = I.index itsl (n - 1) in
   let itsl' = I.prefix itsl (n - 1) in
@@ -1298,7 +1380,7 @@ let lemma_addm_ancestor_is_proving_caseC (itsl: its_log {I.length itsl > 0}):
   let dh' = desc_hash_dir v' d in
 
   lemma_eac_value_is_stored_value itsl' k' tid;
-  //assert(v' = eac_merkle_value itsl' k');                    
+  //assert(v' = eac_merkle_value itsl' k');
 
   lemma_eac_ptrfn itsl' k' d;
   lemma_instore_implies_root_reachable itsl' k' tid;
@@ -1308,7 +1390,7 @@ let lemma_addm_ancestor_is_proving_caseC (itsl: its_log {I.length itsl > 0}):
     //assert(k2 <> k);
     //assert(is_proper_desc k2 k);
     lemma_proper_desc_depth_monotonic k2 k;
-    
+
     //lemma_proper_desc_transitive1 k2 k k';
     //assert(points_to pf k2 k');
     lemma_reachable_between pf k k';
@@ -1333,7 +1415,7 @@ let lemma_addm_ancestor_is_proving_caseD (itsl: its_log {I.length itsl > 0}):
                   let e = I.index itsl (n - 1) in
                   let itsl' = I.prefix itsl (n - 1) in
                   let k = V.key_of e in
-                  AddM?.k' e = proving_ancestor itsl' k)) = 
+                  AddM?.k' e = proving_ancestor itsl' k)) =
   let n = I.length itsl in
   let e = I.index itsl (n - 1) in
   let itsl' = I.prefix itsl (n - 1) in
@@ -1364,7 +1446,7 @@ let lemma_addm_ancestor_is_proving_caseD (itsl: its_log {I.length itsl > 0}):
   let dh' = desc_hash_dir v' d in
 
   lemma_eac_value_is_stored_value itsl' k' tid;
-  //assert(v' = eac_merkle_value itsl' k');                    
+  //assert(v' = eac_merkle_value itsl' k');
 
   lemma_instore_implies_root_reachable itsl' k' tid;
   lemma_proving_ancestor_greatest_depth itsl' k k';
@@ -1383,7 +1465,7 @@ let lemma_addm_ancestor_is_proving_caseD (itsl: its_log {I.length itsl > 0}):
       lemma_reachable_between pf pk k';
       //assert(points_to_some pf k' (desc_dir pk k'));
       lemma_two_ancestors_related k pk (child d k');
-  
+
       if is_desc pk (child d k') then ()
       else (
         //assert(is_proper_desc (child d k') pk);
@@ -1391,10 +1473,10 @@ let lemma_addm_ancestor_is_proving_caseD (itsl: its_log {I.length itsl > 0}):
         lemma_proper_desc_depth_monotonic (child d k') pk
       )
     )
-    else 
+    else
       //assert(is_proper_desc k' pk);
       lemma_proper_desc_depth_monotonic k' pk
-    
+
   )
 
 let lemma_addm_ancestor_is_proving_caseE (itsl: its_log {I.length itsl > 0}):
@@ -1411,7 +1493,7 @@ let lemma_addm_ancestor_is_proving_caseE (itsl: its_log {I.length itsl > 0}):
                      is_proper_desc k k' /\
                      (let d = desc_dir k k' in
                        mv_points_to v' d k))))
-        (ensures False) = 
+        (ensures False) =
   let n = I.length itsl in
   let e = I.index itsl (n - 1) in
   let itsl' = I.prefix itsl (n - 1) in
@@ -1450,7 +1532,7 @@ let lemma_addm_ancestor_is_proving_caseE (itsl: its_log {I.length itsl > 0}):
   lemma_eac_ptrfn itsl' k' d;
   //assert(points_to pf k k');
   lemma_points_to_reachable pf k k';
-  lemma_reachable_transitive pf k k' Root;  
+  lemma_reachable_transitive pf k k' Root;
   ()
 
 let lemma_addm_ancestor_is_proving_caseF (itsl: its_log {I.length itsl > 0}):
@@ -1472,7 +1554,7 @@ let lemma_addm_ancestor_is_proving_caseF (itsl: its_log {I.length itsl > 0}):
                   let e = I.index itsl (n - 1) in
                   let itsl' = I.prefix itsl (n - 1) in
                   let k = V.key_of e in
-                  AddM?.k' e = proving_ancestor itsl' k)) =                        
+                  AddM?.k' e = proving_ancestor itsl' k)) =
   let n = I.length itsl in
   let e = I.index itsl (n - 1) in
   let itsl' = I.prefix itsl (n - 1) in
@@ -1503,7 +1585,7 @@ let lemma_addm_ancestor_is_proving_caseF (itsl: its_log {I.length itsl > 0}):
   let dh' = desc_hash_dir v' d in
 
   lemma_eac_value_is_stored_value itsl' k' tid;
-  //assert(v' = eac_merkle_value itsl' k');                    
+  //assert(v' = eac_merkle_value itsl' k');
 
   lemma_eac_ptrfn itsl' k' d;
   lemma_instore_implies_root_reachable itsl' k' tid;
@@ -1520,7 +1602,7 @@ let lemma_addm_ancestor_is_proving_caseF (itsl: its_log {I.length itsl > 0}):
     else (
       lemma_two_ancestors_related k k' pk;
 
-      if is_desc k' pk then 
+      if is_desc k' pk then
         lemma_proper_desc_depth_monotonic k' pk
       else (
         lemma_reachable_between pf pk k';
@@ -1544,14 +1626,14 @@ let lemma_addm_ancestor_is_proving (itsl: its_log {I.length itsl > 0}):
                   let e = I.index itsl (n - 1) in
                   let itsl' = I.prefix itsl (n - 1) in
                   let k = V.key_of e in
-                  Root <> k /\ AddM?.k' e = proving_ancestor itsl' k)) = 
+                  Root <> k /\ AddM?.k' e = proving_ancestor itsl' k)) =
   let n = I.length itsl in
   let e = I.index itsl (n - 1) in
   let itsl' = I.prefix itsl (n - 1) in
-  let k = V.key_of e in                  
+  let k = V.key_of e in
   let k' = AddM?.k' e in
-  
-  let tid = TL.thread_id_of itsl (n - 1) in  
+
+  let tid = TL.thread_id_of itsl (n - 1) in
 
   (* state of verifier thread tid after processing itsl *)
   let vs = thread_state_post itsl (n - 1) in
@@ -1573,7 +1655,7 @@ let lemma_addm_ancestor_is_proving (itsl: its_log {I.length itsl > 0}):
 
   (* k' is in the verifier store since vaddm checks this *)
   assert(store_contains st' k');
-  
+
   let v' = to_merkle_value (V.stored_value st' k') in
   let d = desc_dir k k' in
   let dh' = desc_hash_dir v' d in
@@ -1582,22 +1664,22 @@ let lemma_addm_ancestor_is_proving (itsl: its_log {I.length itsl > 0}):
 
   if root_reachable itsl' k then (
     match dh' with
-    | Empty -> 
+    | Empty ->
       lemma_addm_ancestor_is_proving_caseA itsl
-    | Desc k2 _ _ -> 
-      if k2 = k then lemma_addm_ancestor_is_proving_caseB itsl        
+    | Desc k2 _ _ ->
+      if k2 = k then lemma_addm_ancestor_is_proving_caseB itsl
       else lemma_addm_ancestor_is_proving_caseC itsl
-  )  
+  )
   else (
     match dh' with
     | Empty -> lemma_addm_ancestor_is_proving_caseD itsl
-    | Desc k2 _ _ -> 
+    | Desc k2 _ _ ->
       if k2 = k then lemma_addm_ancestor_is_proving_caseE itsl
       else lemma_addm_ancestor_is_proving_caseF itsl
   )
 
 (* if the store contains a k, it contains its proving ancestor *)
-let lemma_store_contains_proving_ancestor (itsl: TL.eac_log) 
+let lemma_store_contains_proving_ancestor (itsl: TL.eac_log)
   (tid:TL.valid_tid itsl) (k:key{k <> Root}):
   Lemma (store_contains (TL.thread_store itsl tid) k ==>
          store_contains (TL.thread_store itsl tid)
